Parikh/Pilling_Lemma.thy
@@ -1,0 +1,200 @@
+theory Pilling_Lemma
+  imports
+    Lfun
+    Eq_Sys
+begin
+
+section \<open>The lemma from Pilling's paper\<close>
+
+(* In this section, the lemma from Pilling's paper will be proved.
+   For some reason, the lemma will not be needed in the further proof.
+*)
+
+
+subsection \<open>g_pre (in the paper g_{iN} resp. X_{iN}\<close>
+
+fun g_pre :: "'a eq_sys \<Rightarrow> nat \<Rightarrow> nat \<Rightarrow> 'a lfun" where
+  "g_pre _ _ 0 = N {}" |
+  "g_pre f_sys i (Suc n) = subst (f_sys ! i) (\<lambda>j. if j < length f_sys then g_pre f_sys j n else V j)"
+
+
+lemma g_pre_eval:
+  assumes "\<forall>j < length f_sys. s' j = eval (g_pre f_sys j n) s"
+      and "\<forall>j \<ge> length f_sys. s' j = s j"
+    shows "eval (g_pre f_sys i (Suc n)) s = eval (f_sys ! i) s'"
+using assms by (simp add: substitution_lemma)
+
+
+lemma g_pre_monotonically_increasing:
+  "eval (g_pre f_sys i n) s \<subseteq> eval (g_pre f_sys i (Suc n)) s"
+proof (induction n arbitrary: i)
+  case 0
+  then show ?case by auto
+next
+  case (Suc n)
+  let ?s = "\<lambda>j. if j < length f_sys then eval (g_pre f_sys j n) s else s j"
+  let ?s_Suc = "\<lambda>j. if j < length f_sys then eval (g_pre f_sys j (Suc n)) s else s j"
+  from Suc.IH have s_subseteq_s_Suc: "?s j \<subseteq> ?s_Suc j" for j by auto
+
+  have "eval (g_pre f_sys i (Suc n)) s = eval (f_sys ! i) ?s" using g_pre_eval[of f_sys] by auto
+  also have "\<dots> \<subseteq> eval (f_sys ! i) ?s_Suc" using s_subseteq_s_Suc lfun_mono_aux[where s="?s"] by auto
+  also have "\<dots> = eval (g_pre f_sys i (Suc (Suc n))) s" using g_pre_eval[of f_sys ?s_Suc] by auto
+  finally show ?case .
+qed
+
+
+lemma g_pre_subseteq_sol:
+  assumes "i < length f_sys"
+      and "solves_ineq_sys f_sys s"
+    shows "eval (g_pre f_sys i n) s \<subseteq> eval (f_sys ! i) s"
+using assms proof (induction n arbitrary: i)
+  case 0
+  then show ?case by auto
+next
+  case (Suc n)
+  let ?s' = "\<lambda>j. if j < length f_sys then eval (g_pre f_sys j n) s else s j"
+
+  have "?s' j \<subseteq> s j" for j
+  proof (cases "j < length f_sys")
+    case True
+    with Suc have "?s' j \<subseteq> eval (f_sys ! j) s" by auto
+    also have "\<dots> \<subseteq> s j" using assms(2) True unfolding solves_ineq_sys_def by auto
+    finally show ?thesis .
+  next
+    case False
+    then show ?thesis by auto
+  qed
+  then have "eval (f_sys ! i) ?s' \<subseteq> eval (f_sys ! i) s" using lfun_mono_aux by meson
+  then show ?case using g_pre_eval[of f_sys ?s'] by auto
+qed
+
+
+lemma g_pre_indep:
+  assumes "i < length f_sys"
+  shows "\<forall>x \<in> vars (g_pre f_sys i n). x \<ge> length f_sys"
+proof (induction n arbitrary: i)
+  case 0
+  then show ?case by auto
+next
+  case (Suc n)
+  let ?upd = "\<lambda>x. if x < length f_sys then g_pre f_sys x n else V x"
+  from vars_subst_upper have "vars (g_pre f_sys i (Suc n)) \<subseteq> (\<Union>x. vars (?upd x))" by simp
+  moreover have "\<forall>y \<in> vars (?upd x). y \<ge> length f_sys" for x using Suc by simp
+  ultimately show ?case by auto
+qed
+
+
+
+subsection \<open>g\<close>
+
+(* This is the only reason why we have included the countable union in the lfun definition *)
+definition g :: "'a eq_sys \<Rightarrow> nat \<Rightarrow> 'a lfun" where
+  "g f_sys i \<equiv> UnionC (\<lambda>n. g_pre f_sys i n)"
+
+
+lemma g_indep:
+  assumes "i < length f_sys"
+  shows "\<forall>x \<in> vars (g f_sys i). x \<ge> length f_sys"
+unfolding g_def using assms g_pre_indep by auto
+
+
+lemma solves_g_if_solves_f_ineq:
+  assumes "i < length f_sys"
+      and "solves_ineq_sys f_sys s"
+    shows "eval (g f_sys i) s \<subseteq> eval (f_sys ! i) s"
+unfolding g_def proof
+  fix x
+  assume "x \<in> eval (UnionC (g_pre f_sys i)) s"
+  then show "x \<in> eval (f_sys ! i) s" using g_pre_subseteq_sol[OF assms] by auto
+qed
+
+
+lemma Union_index_shift: "(\<Union>n. f n) = f 0 \<union> (\<Union>n. f (Suc n))"
+proof
+  show "\<Union> (range f) \<subseteq> f 0 \<union> (\<Union>n. f (Suc n))"
+  proof
+    fix x
+    assume "x \<in> \<Union> (range f)"
+    then obtain n where x_in_f: "n \<ge> 0 \<and> x \<in> f n" by auto
+    show "x \<in> f 0 \<union> (\<Union>n. f (Suc n))"
+    proof (cases "n=0")
+      case True
+      with x_in_f show ?thesis by auto
+    next
+      case False
+      with x_in_f have "\<exists>n'. Suc n' = n" by presburger
+      then obtain n' where "Suc n' = n" by blast
+      with x_in_f show ?thesis by auto
+    qed
+  qed
+  show "f 0 \<union> (\<Union>n. f (Suc n)) \<subseteq> \<Union> (range f)" by auto
+qed
+
+
+lemma g_pre_g_Union: "(\<Union>n. eval (g_pre f_sys i (Suc n)) s) =
+  eval (subst (f_sys ! i) (\<lambda>i. if i < length f_sys then g f_sys i else V i)) s"
+proof -
+  let ?s = "(\<lambda>n j. if j < length f_sys then eval (g_pre f_sys j n) s else s j)"
+  have "?s n j \<subseteq> ?s (Suc n) j" for n j
+    using g_pre_monotonically_increasing by fastforce
+  then have s_monotone: "\<forall>n. ?s n \<le> ?s (Suc n)" by (simp add: le_fun_def)
+
+  have s_Union: "(\<Union>i. if x < length f_sys then eval (g_pre f_sys x i) s else s x) =
+    (if x < length f_sys then eval (g f_sys x) s else s x)" for x
+    unfolding g_def by simp
+
+  have "eval (g_pre f_sys i (Suc n)) s = eval (f_sys ! i) (?s n)" for n
+    using g_pre_eval[of f_sys] by auto
+  then have "(\<Union>n. eval (g_pre f_sys i (Suc n)) s) = (\<Union>n. eval (f_sys ! i) (?s n))" by auto
+  also have "\<dots> = eval (f_sys ! i) (\<lambda>x. \<Union>i. if x < length f_sys then eval (g_pre f_sys x i) s else s x)"
+    using s_monotone lfun_cont[of ?s "f_sys ! i"] by argo
+  also have "\<dots> = eval (f_sys ! i) (\<lambda>x. if x < length f_sys then eval (g f_sys x) s else s x)"
+    using s_Union by simp
+  also have "\<dots> = eval (subst (f_sys ! i) (\<lambda>i. if i < length f_sys then g f_sys i else V i)) s"
+    using substitution_lemma[of "\<lambda>x. if x < length f_sys then eval (g f_sys x) s else s x"
+                                "\<lambda>i. if i < length f_sys then g f_sys i else V i"]
+    by fastforce
+  finally show ?thesis .
+qed
+
+
+lemma solves_f_if_solves_g_eq:
+  assumes "\<forall>i < length f_sys. eval (g f_sys i) s = s i"
+  shows "solves_eq_sys f_sys s"
+unfolding solves_eq_sys_def proof (standard, standard)
+  fix i
+  assume "i < length f_sys"
+  with assms(1) have "s i = (\<Union>n. eval (g_pre f_sys i n) s)" unfolding g_def by auto
+  also have "\<dots> = (\<Union>n. eval (g_pre f_sys i (Suc n)) s)"
+    using Union_index_shift[of "\<lambda>n. eval (g_pre f_sys i n) s"] by auto
+  also have "\<dots> = eval (f_sys ! i) s"
+    using g_pre_g_Union[of f_sys] assms by (simp add: substitution_lemma)
+  finally show "eval (f_sys ! i) s = s i" by auto
+qed
+
+
+(* The lemma from Pilling's paper *)
+lemma lemma_paper:
+  assumes "\<forall>eq \<in> set f_sys. regular_fun eq"
+    shows "\<exists>g_sys. length g_sys = length f_sys \<and> indep_leq g_sys (length f_sys - 1)
+                \<and> (\<forall>s. solves_ineq_sys f_sys s \<longrightarrow> solves_ineq_sys g_sys s)
+                \<and> (\<forall>s. solves_eq_sys g_sys s \<longrightarrow> solves_eq_sys f_sys s)"
+proof -
+  let ?g_sys = "map (\<lambda>i. g f_sys i) [0..<length f_sys]"
+  have length_g_sys: "length ?g_sys = length f_sys" by auto
+  have indep_g_sys: "indep_leq ?g_sys (length f_sys - 1)"
+    unfolding indep_leq_def using g_indep by fastforce
+
+  have "\<lbrakk> i < length f_sys; solves_ineq_sys f_sys s \<rbrakk> \<Longrightarrow> eval (?g_sys ! i) s \<subseteq> s i" for s i
+    using solves_g_if_solves_f_ineq solves_ineq_sys_def by fastforce
+  then have g_sol_of_f: "solves_ineq_sys f_sys s \<longrightarrow> solves_ineq_sys ?g_sys s" for s
+    using solves_ineq_sys_def by (metis length_g_sys)
+
+  have f_sol_of_g: "solves_eq_sys ?g_sys s \<longrightarrow> solves_eq_sys f_sys s" for s
+    using solves_f_if_solves_g_eq solves_eq_sys_def
+    by (metis add_0 diff_zero length_g_sys nth_map_upt)
+
+  from length_g_sys indep_g_sys g_sol_of_f f_sol_of_g show ?thesis by blast
+qed
+
+end
